pcuic/theories/PCUICContextReduction.v
@@ -1,0 +1,116 @@
+(* Distributed under the terms of the MIT license. *)
+From MetaCoq.Template Require Import config utils.
+From MetaCoq.PCUIC Require Import PCUICAst PCUICAstUtils
+     PCUICLiftSubst PCUICEquality PCUICUnivSubst PCUICInduction 
+     PCUICContextRelation PCUICReduction PCUICCases PCUICWeakening.
+
+Require Import ssreflect.
+Require Import Equations.Prop.DepElim.
+From Equations.Type Require Import Relation Relation_Properties.
+From Equations Require Import Equations.
+Set Equations Transparent.
+Set Default Goal Selector "!".
+
+Section CtxReduction.
+  Context {cf : checker_flags}.
+  Context {Σ : global_env}.
+  Context (wfΣ : wf Σ).
+
+  Lemma weakening_red_0 Γ Γ' M N n :
+    n = #|Γ'| ->
+    red Σ Γ M N ->
+    red Σ (Γ ,,, Γ') (lift0 n M) (lift0 n N).
+  Proof. now move=> ->; apply (weakening_red Σ Γ [] Γ'). Qed.
+
+
+  Lemma red_red_ctx Γ Δ t u :
+    red Σ Γ t u ->
+    red_ctx Δ Γ ->
+    red Σ Δ t u.
+  Proof.
+    move=> H Hctx. induction H.
+    revert Δ Hctx.
+    induction r using red1_ind_all; intros Δ Hctx; try solve [eapply red_step; repeat (constructor; eauto)].
+    - red in Hctx.
+      eapply nth_error_pred1_ctx in Hctx; eauto.
+      destruct Hctx as [x' [? ?]].
+      eapply red_step. constructor. eauto.
+      rewrite -(firstn_skipn (S i) Δ).
+      eapply weakening_red_0; auto.
+      rewrite firstn_length_le //.
+      destruct (nth_error Δ) eqn:Heq => //.
+      eapply nth_error_Some_length in Heq. lia.
+    - repeat econstructor; eassumption.
+    - repeat econstructor; eassumption.
+    - repeat econstructor; eassumption.
+    - repeat econstructor; eassumption.
+    - eapply red_abs_alt. eauto. eauto.
+    - eapply red_abs_alt. eauto. apply (IHr (Δ ,, vass na N)).
+      constructor; auto. red. auto.
+    - eapply red_letin; eauto.
+    - eapply red_letin; eauto.
+    - eapply red_letin_alt; eauto.
+      eapply (IHr (Δ ,, vdef na b t)). constructor; eauto.
+      red. split; eauto.
+    - eapply red_case; eauto. unfold on_Trel; pcuic.
+    - eapply red_case; eauto. unfold on_Trel; pcuic.
+    - eapply red_case; eauto. unfold on_Trel; pcuic.
+      eapply OnOne2_All2; eauto. simpl. intuition eauto.
+    - eapply red_proj_c; eauto.
+    - eapply red_app; eauto.
+    - eapply red_app; eauto.
+    - eapply red_prod_alt; eauto.
+    - eapply red_prod_alt; eauto. apply (IHr (Δ ,, vass na M1)); constructor; auto.
+      red; eauto.
+    - eapply red_evar.
+      eapply OnOne2_All2; simpl; eauto. simpl. intuition eauto.
+    - eapply red_fix_one_ty.
+      eapply OnOne2_impl ; eauto.
+      intros [? ? ? ?] [? ? ? ?] [[r ih] e]. simpl in *.
+      inversion e. subst. clear e.
+      split ; auto.
+    - eapply red_fix_one_body.
+      eapply OnOne2_impl ; eauto.
+      intros [? ? ? ?] [? ? ? ?] [[r ih] e]. simpl in *.
+      inversion e. subst. clear e.
+      split ; auto.
+      eapply ih.
+      clear - Hctx. induction (fix_context mfix0).
+      + assumption.
+      + simpl. destruct a as [na [b|] ty].
+        * constructor ; pcuicfo (hnf ; auto).
+        * constructor ; pcuicfo (hnf ; auto).
+    - eapply red_cofix_one_ty.
+      eapply OnOne2_impl ; eauto.
+      intros [? ? ? ?] [? ? ? ?] [[r ih] e]. simpl in *.
+      inversion e. subst. clear e.
+      split ; auto.
+    - eapply red_cofix_one_body.
+      eapply OnOne2_impl ; eauto.
+      intros [? ? ? ?] [? ? ? ?] [[r ih] e]. simpl in *.
+      inversion e. subst. clear e.
+      split ; auto.
+      eapply ih.
+      clear - Hctx. induction (fix_context mfix0).
+      + assumption.
+      + simpl. destruct a as [na [b|] ty].
+        * constructor ; pcuicfo (hnf ; auto).
+        * constructor ; pcuicfo (hnf ; auto).
+    - auto.
+    - eapply red_trans; eauto.
+  Qed.
+
+  
+Lemma red_ctx_rel_red_context_rel Σ Γ : 
+  CRelationClasses.relation_equivalence (red_ctx_rel Σ Γ) (red_context_rel Σ Γ).
+Proof.
+  rewrite /red_ctx_rel /red_context_rel; split.
+  - induction 1.
+    * admit.
+    * eapply context_relation_refl => Δ [na [b|] ty]; constructor; auto; constructor 2.
+    * eapply context_relation_trans; eauto.
+      intros.
+      depelim X4; depelim X5; constructor; etransitivity; eauto.
+
+
+
